@prefix ldes: <https://w3id.org/ldes#> .
@prefix tree: <https://w3id.org/tree#> .
@prefix cc: <http://creativecommons.org/ns#> .
@prefix dct: <http://purl.org/dc/terms/> .
@prefix foaf: <http://xmlns.com/foaf/0.1/> .
@prefix gsp: <http://www.opengis.net/ont/geosparql#> .
@prefix locn: <http://www.w3.org/ns/locn#> .
@prefix owl: <http://www.w3.org/2002/07/owl#> .
@prefix prov: <http://www.w3.org/ns/prov#> .
@prefix rdf: <http://www.w3.org/1999/02/22-rdf-syntax-ns#> .
@prefix rdfs: <http://www.w3.org/2000/01/rdf-schema#> .
@prefix schema: <http://schema.org/> .
@prefix sh: <http://www.w3.org/ns/shacl#> .
@prefix voaf: <http://purl.org/vocommons/voaf#> .
@prefix vs: <http://www.w3.org/2003/06/sw-vocab-status/ns#> .
@prefix wdrs: <http://www.w3.org/2007/05/powder-s#> .
@prefix xhtm: <http://www.w3.org/1999/xhtml> .
@prefix xml: <http://www.w3.org/XML/1998/namespace> .
@prefix xsd: <http://www.w3.org/2001/XMLSchema#> .
@prefix hydra: <http://www.w3.org/ns/hydra/core#>.

ldes: a foaf:Document ;
      foaf:primaryTopic ldes:Vocabulary ;
      cc:license <http://creativecommons.org/licenses/by/4.0/>;
      dct:creator <https://pietercolpaert.be/#me> .

<https://pietercolpaert.be/#me> foaf:name "Pieter Colpaert"; foaf:mbox "pieter.colpaert@ugent.be".

ldes:Vocabulary a owl:Ontology ;
                rdfs:label "The Linked Data Event Streams specification"@en;
                rdfs:comment "A hypermedia specification for maintaining a collection with immutable members."@en.

ldes:EventStream a rdfs:Class ;
                 rdfs:subClassOf tree:Collection ;
                 rdfs:label "Event Stream"@en;
                 rdfs:comment "An Event Stream is a tree:Collection containing immutable members."@en .

ldes:EventSource rdfs:subClassOf tree:ViewDescription ;
                 rdfs:label "Event Source"@en ;
                 rdfs:comment "A data service that provides the source other views should synchronize with"@en .

ldes:RetentionPolicy a rdf:Class ;
                     rdfs:label "Retention Policy"@en ;
                     rdfs:comment "The abstract concept of a retention policy."@en .

ldes:LatestVersionSubset rdfs:subClassOf ldes:RetentionPolicy ;   
                         rdfs:label "Latest Version Subset Policy"@en ;
                         rdfs:comment "The latest version of the element."@en .
                         
ldes:DurationAgoPolicy rdfs:subClassOf ldes:RetentionPolicy ;   
                       rdfs:label "Time-based Retention Policy"@en ;
                       rdfs:comment "Retention policy based on a member’s timestamp and a duration."@en .

ldes:PointInTimePolicy rdfs:subClassOf ldes:RetentionPolicy ;
                       rdfs:label "Point in Time Retention Policy"@en ;
                       rdfs:comment "Retention policy based on a member’s timestamp and a given point in time."@en .

ldes:retentionPolicy a rdf:Property ;
                     rdfs:label "has retention policy"@en;
                     rdfs:comment "Links to a retention policy."@en ;
                     rdfs:domain tree:ViewDescription ;
                     rdfs:range ldes:RetentionPolicy .

ldes:amount a rdf:Property ;
            rdfs:label "amount"@en;
            rdfs:comment "Amount of versions to keep."@en ;
            rdfs:range xsd:nonNegativeInteger ;
            rdfs:domain ldes:LastVersionSubset .

ldes:pointInTime a rdf:Property ;
                 rdfs:label "point in time"@en;
                 rdfs:comment "After this point in time members are kept."@en ;
                 rdfs:range xsd:dateTime ;
                 rdfs:domain ldes:PointInTimePolicy .

ldes:versionKey a rdf:Property ;
                rdfs:label "version key"@en;
                rdfs:comment "A list of SHACL property paths to compose a version key."@en ;
                rdfs:range rdf:List ;
                rdfs:domain ldes:LastVersionSubset .

ldes:versionOfPath a rdf:Property ;
                   rdfs:label "versionOf Path"@en;
                   rdfs:comment "SHACL property path to the non-versioned identifier of the entity."@en .


ldes:timestampPath a rdf:Property ;
                   rdfs:label "Timestamp Path"@en;
                   rdfs:comment "SHACL property path to the timestamp when the version object entered the event stream."@en .

ldes:versionMaterializationOf a rdf:Property ;
                   rdfs:label "Version Materialization Of"@en;
                   rdfs:comment "Links to the original LDES"@en ;
                   rdfs:range ldes:EventStream ;
                   rdfs:domain tree:Collection .

ldes:versionMaterializationUntil a rdf:Property ;
                   rdfs:label "Version Materialization Until"@en;
                   rdfs:comment "Timestamp until versions were processed"@en ;
                   rdfs:range xsd:dateTime ;
                   rdfs:domain tree:Collection .